MLS.Bytes.fsti
@@ -6,10 +6,12 @@ type nat_lbytes (sz:nat) = n:nat{n < pow2 (8*sz)}
 
 /// Minimal interface to manipulate symbolic bytes.
 /// Here are the explanations for a few design decisions:
-/// - `slice` returns an option, hence can fail if the indexes are not on the correct bounds.
-///   * We require `slice` to succeed on the bounds of a `concat` (see `slice_concat_...`).
-///   * This is useful to state the `concat_slice` lemma in a way which would be correct on symbolic bytes.
 /// - We don't require that only `empty` has length zero, e.g. we may have `concat empty empty <> empty`.
+/// - We implement `split` and not `slice`, because `slice` causes trouble in the symbolic case:
+///   with `slice`, how do you get the left and right part of `concat empty (concat empty empty)`?
+/// - `split` returns an option, hence can fail if the indexes are not on the correct bounds.
+///   * We require `split` to succeed on the bound of a `concat` (see `split_concat_...`).
+///   * This is useful to state the `concat_split` lemma in a way which would be correct on symbolic bytes.
 /// - To compensate the last fact, and the fact that we don't require decidable equality,
 ///   we need a function that recognize the `empty` bytes.
 /// - The `to_nat` function can fail, if the bytes are not public for example
@@ -24,23 +26,20 @@ class bytes_like (bytes:Type0) = {
   concat: bytes -> bytes -> bytes;
   concat_length: b1:bytes -> b2:bytes -> Lemma (length (concat b1 b2) == (length b1) + (length b2));
 
-  slice: b:bytes -> i:nat -> j:nat{i <= j /\ j <= length b} -> option bytes;
-  slice_length: b:bytes -> i:nat -> j:nat{i <= j /\ j <= length b} -> Lemma (
-    match slice b i j with
-    | Some res -> length res == j-i
+  split: b:bytes -> i:nat{i <= length b} -> option (bytes & bytes);
+  split_length: b:bytes -> i:nat{i <= length b} -> Lemma (
+    match split b i with
+    | Some (b1, b2) -> length b1 == i /\ i+length b2 == length b
     | None -> True
   );
 
-  slice_concat_left: b1:bytes -> b2:bytes -> Lemma
+  split_concat: b1:bytes -> b2:bytes -> Lemma
     (requires (length b1) <= (length (concat b1 b2)))
-    (ensures slice (concat b1 b2) 0 (length b1)  == Some b1);
-  slice_concat_right: b1:bytes -> b2:bytes -> Lemma
-    (requires (length b1) <= (length (concat b1 b2)))
-    (ensures slice (concat b1 b2) (length b1) (length (concat b1 b2)) == Some b2);
+    (ensures split (concat b1 b2) (length b1) == Some (b1, b2));
 
-  concat_slice: b:bytes -> i:nat{i <= length b} -> Lemma (
-    match slice b 0 i, slice b i (length b) with
-    | Some lhs, Some rhs -> concat lhs rhs == b
+  concat_split: b:bytes -> i:nat{i <= length b} -> Lemma (
+    match split b i with
+    | Some (lhs, rhs) -> concat lhs rhs == b
     | _ -> True
   );
 
@@ -64,7 +63,7 @@ type bytes_compatible_pre (bytes:Type0) {|bytes_like bytes|} =
   pre:(bytes -> Type0){
     (pre empty) /\
     (forall b1 b2. pre b1 /\ pre b2 ==> pre (concat b1 b2)) /\
-    (forall b i j. pre b /\ Some? (slice b i j) ==> pre (Some?.v (slice b i j))) /\
+    (forall b i. pre b /\ Some? (split b i) ==> pre (fst (Some?.v (split b i))) /\ pre (snd (Some?.v (split b i)))) /\
     (forall sz n. pre (from_nat sz n))
   }
 
